Update std lib and etcd-raft translations
etcd-raft wasn't part of ci-goose-check.py, and the standard library
packages were only translated as part of that invocation. This allowed
both translations to get out-of-date.

This commit:

1. Separates the standard library translation from etcd-raft.
2. Updates ci-goose-check.py to keep both standard library and etcd-raft
   up-to-date.
3. Adapts to a small change in sync.WaitGroup (it now calls
   `runtime_SemacquireWaitGroup` which has the same runtime behavior as
   `runtime_Semacquire` but provides better debugging).

new/trusted_code/sync.v
@@ -69,6 +69,11 @@ Definition runtime_Semacquire : val :=
     )
 .
 
+(* differs from runtime_Semacquire only in the park "reason", used for internal
+concurrency testing *)
+Definition runtime_SemacquireWaitGroup : val :=
+  λ: "addr", func_call #pkg_name' #"runtime_Semacquire" "addr".
+
 Definition runtime_Semrelease : val :=
   λ: <>, #() #(). (* FIXME: use `AtomicAdd` *)
 
