new/code/os.v
@@ -6,8 +6,6 @@ Section code.
 Context `{ffi_syntax}.
 
 
-Axiom dirBufPool'init : val.
-
 Axiom ErrInvalid'init : val.
 
 Axiom ErrPermission'init : val.
@@ -28,6 +26,10 @@ Axiom Interrupt'init : val.
 
 Axiom Kill'init : val.
 
+Axiom initCwd'init : val.
+
+Axiom initCwdErr'init : val.
+
 Axiom Stdin'init : val.
 
 Axiom Stdout'init : val.
@@ -36,17 +38,13 @@ Axiom Stderr'init : val.
 
 Axiom errWriteAtInAppendMode'init : val.
 
+Axiom errPathEscapes'init : val.
+
 Axiom lstat'init : val.
 
 Axiom checkWrapErr'init : val.
 
-Axiom checkPidfdOnce'init : val.
-
 Axiom errPatternHasSeparator'init : val.
-
-Axiom pollCopyFileRange'init : val.
-
-Axiom pollSplice'init : val.
 
 Definition pkg_name' : go_string := "os".
 
@@ -61,8 +59,7 @@ Axiom _'init : val.
 Definition initialize' : val :=
   rec: "initialize'" <> :=
     globals.package_init pkg_name' vars' functions' msets' (λ: <>,
-      exception_do (do:  (dirBufPool'init #());;;
-      do:  (ErrInvalid'init #());;;
+      exception_do (do:  (ErrInvalid'init #());;;
       do:  (ErrPermission'init #());;;
       do:  (ErrExist'init #());;;
       do:  (ErrNotExist'init #());;;
@@ -76,12 +73,11 @@ Definition initialize' : val :=
       do:  (Stdout'init #());;;
       do:  (Stderr'init #());;;
       do:  (errWriteAtInAppendMode'init #());;;
+      do:  (errPathEscapes'init #());;;
       do:  (lstat'init #());;;
       do:  (checkWrapErr'init #());;;
-      do:  (checkPidfdOnce'init #());;;
-      do:  (errPatternHasSeparator'init #());;;
-      do:  (pollCopyFileRange'init #());;;
-      do:  (pollSplice'init #()))
+      do:  (initCwd'init #());;;
+      do:  (errPatternHasSeparator'init #()))
       ).
 
 End code.
